Start adding compartments to backend
The general strategy consists in adding compartments to all memory
operations, assigning one more more variables in as direct a manner as
possible, considering in particular the correspondence between
compartments in the assumptions and compartments in the conclusions.
While doing so, catalogue the unsolved goals and consider strategies
for discharging them efficiently. So far, nothing looks problematic or
difficult.

backend/Cminor.v
@@ -379,9 +379,9 @@ Inductive eval_expr: expr -> val -> Prop :=
       eval_expr a2 v2 ->
       eval_binop op v1 v2 m = Some v ->
       eval_expr (Ebinop op a1 a2) v
-  | eval_Eload: forall chunk addr vaddr v,
+  | eval_Eload: forall chunk addr vaddr cp v,
       eval_expr addr vaddr ->
-      Mem.loadv chunk m vaddr = Some v ->
+      Mem.loadv chunk m vaddr cp = Some v ->
       eval_expr (Eload chunk addr) v.
 
 Inductive eval_exprlist: list expr -> list val -> Prop :=
@@ -450,9 +450,9 @@ Inductive step: state -> trace -> state -> Prop :=
   | step_skip_block: forall f k sp e m,
       step (State f Sskip (Kblock k) sp e m)
         E0 (State f Sskip k sp e m)
-  | step_skip_call: forall f k sp e m m',
+  | step_skip_call: forall f k sp e m cp m',
       is_call_cont k ->
-      Mem.free m sp 0 f.(fn_stackspace) = Some m' ->
+      Mem.free m sp 0 f.(fn_stackspace) cp = Some m' ->
       step (State f Sskip k (Vptr sp Ptrofs.zero) e m)
         E0 (Returnstate Vundef k m')
 
@@ -461,10 +461,10 @@ Inductive step: state -> trace -> state -> Prop :=
       step (State f (Sassign id a) k sp e m)
         E0 (State f Sskip k sp (PTree.set id v e) m)
 
-  | step_store: forall f chunk addr a k sp e m vaddr v m',
+  | step_store: forall f chunk addr a k sp e m vaddr v cp m',
       eval_expr sp e m addr vaddr ->
       eval_expr sp e m a v ->
-      Mem.storev chunk m vaddr v = Some m' ->
+      Mem.storev chunk m vaddr v cp = Some m' ->
       step (State f (Sstore chunk addr a) k sp e m)
         E0 (State f Sskip k sp e m')
 
@@ -477,7 +477,7 @@ Inductive step: state -> trace -> state -> Prop :=
       step (State f (Scall optid sig a bl) k sp e m)
         E0 (Callstate fd vargs (Kcall optid f sp e k) m)
 
-  | step_tailcall: forall f sig a bl k sp e m vf vargs fd m',
+  | step_tailcall: forall f sig a bl k sp e m vf vargs fd cp m',
       eval_expr (Vptr sp Ptrofs.zero) e m a vf ->
       eval_exprlist (Vptr sp Ptrofs.zero) e m bl vargs ->
       Genv.find_funct ge vf = Some fd ->
@@ -485,7 +485,7 @@ Inductive step: state -> trace -> state -> Prop :=
       forall (COMP: comp_of fd = f.(fn_comp)),
       forall (ALLOWED: needs_calling_comp f.(fn_comp) = false),
       forall (ALLOWED': Policy.allowed_call pol f.(fn_comp) fd),
-      Mem.free m sp 0 f.(fn_stackspace) = Some m' ->
+      Mem.free m sp 0 f.(fn_stackspace) cp = Some m' ->
       step (State f (Stailcall sig a bl) k (Vptr sp Ptrofs.zero) e m)
         E0 (Callstate fd vargs (call_cont k) m')
 
@@ -529,13 +529,13 @@ Inductive step: state -> trace -> state -> Prop :=
       step (State f (Sswitch islong a cases default) k sp e m)
         E0 (State f (Sexit (switch_target n default cases)) k sp e m)
 
-  | step_return_0: forall f k sp e m m',
-      Mem.free m sp 0 f.(fn_stackspace) = Some m' ->
+  | step_return_0: forall f k sp e m cp m',
+      Mem.free m sp 0 f.(fn_stackspace) cp = Some m' ->
       step (State f (Sreturn None) k (Vptr sp Ptrofs.zero) e m)
         E0 (Returnstate Vundef (call_cont k) m')
-  | step_return_1: forall f a k sp e m v m',
+  | step_return_1: forall f a k sp e m v cp m',
       eval_expr (Vptr sp Ptrofs.zero) e m a v ->
-      Mem.free m sp 0 f.(fn_stackspace) = Some m' ->
+      Mem.free m sp 0 f.(fn_stackspace) cp = Some m' ->
       step (State f (Sreturn (Some a)) k (Vptr sp Ptrofs.zero) e m)
         E0 (Returnstate v (call_cont k) m')
 
@@ -619,8 +619,12 @@ Proof.
 - congruence.
 - assert (v0 = v1) by eauto. congruence.
 - assert (v0 = v1) by eauto. assert (v3 = v2) by eauto. congruence.
-- assert (vaddr0 = vaddr) by eauto. congruence.
-Qed.
+- assert (vaddr0 = vaddr) by eauto.
+  (* congruence. *)
+  subst.
+  admit. (* RB: NOTE: Component determinism of successful [loadv]s *)
+(* Qed. *)
+Admitted.
 
 Lemma eval_exprlist_determ:
   forall ge sp e m al vl, eval_exprlist ge sp e m al vl ->
@@ -653,11 +657,16 @@ Proof.
   intros. constructor; set (ge := Genv.globalenv p); simpl; intros.
 - (* determ *)
   inv H; inv H0; Determ.
+  + admit. (* RB: NOTE: Compartment determinacy of [free] *)
+  + subst. admit. (* RB: NOTE: Compartment determinacy of [storev] *)
+  + admit. (* RB: NOTE: Compartment determinacy of [free] *)
   + subst vargs0. exploit external_call_determ. eexact H2.  eexact H13.
     intros (A & B). split; intros; auto.
     apply B in H; destruct H; congruence.
   + subst v0. assert (b0 = b) by (inv H2; inv H13; auto). subst b0; auto.
   + assert (n0 = n) by (inv H2; inv H14; auto). subst n0; auto.
+  + admit. (* RB: NOTE: Compartment determinacy of [free] *)
+  + admit. (* RB: NOTE: Compartment determinacy of [free] *)
   + exploit external_call_determ. eexact H1. eexact H7.
     intros (A & B). split; intros; auto.
     apply B in H; destruct H; congruence.
@@ -670,7 +679,8 @@ Proof.
   red; intros; red; intros. inv H; inv H0.
 - (* final states *)
   inv H; inv H0; auto.
-Qed.
+(* Qed. *)
+Admitted.
 
 (** * Alternate operational semantics (big-step) *)
 
@@ -716,10 +726,10 @@ Definition outcome_result_value
   end.
 
 Definition outcome_free_mem
-    (out: outcome) (m: mem) (sp: block) (sz: Z) (m': mem) :=
+    (out: outcome) (m: mem) (sp: block) (sz: Z) (cp: compartment) (m': mem) :=
   match out with
   | Out_tailcall_return _ => m' = m
-  | _ => Mem.free m sp 0 sz = Some m'
+  | _ => Mem.free m sp 0 sz cp = Some m'
   end.
 
 Section NATURALSEM.
@@ -738,12 +748,12 @@ Inductive eval_funcall:
         mem -> fundef -> list val -> trace ->
         mem -> val -> Prop :=
   | eval_funcall_internal:
-      forall cp m f vargs m1 sp e t e2 m2 out vres m3,
+      forall cp m f vargs m1 sp e t e2 m2 out vres cp' m3,
       Mem.alloc m f.(fn_comp) 0 f.(fn_stackspace) = (m1, sp) ->
       set_locals f.(fn_vars) (set_params vargs f.(fn_params)) = e ->
       exec_stmt f (Vptr sp Ptrofs.zero) e m1 f.(fn_body) t e2 m2 out ->
       outcome_result_value out vres ->
-      outcome_free_mem out m2 sp f.(fn_stackspace) m3 ->
+      outcome_free_mem out m2 sp f.(fn_stackspace) cp' m3 ->
       eval_funcall cp m (Internal f) vargs t m3 vres
   | eval_funcall_external:
       forall ef cp m args t res m',
@@ -770,10 +780,10 @@ with exec_stmt:
       eval_expr ge sp e m a v ->
       exec_stmt f sp e m (Sassign id a) E0 (PTree.set id v e) m Out_normal
   | exec_Sstore:
-      forall f sp e m chunk addr a vaddr v m',
+      forall f sp e m chunk addr a vaddr v cp m',
       eval_expr ge sp e m addr vaddr ->
       eval_expr ge sp e m a v ->
-      Mem.storev chunk m vaddr v = Some m' ->
+      Mem.storev chunk m vaddr v cp = Some m' ->
       exec_stmt f sp e m (Sstore chunk addr a) E0 e m' Out_normal
   | exec_Scall:
       forall f sp e m optid sig a bl vf vargs fd t m' vres e',
@@ -840,7 +850,7 @@ with exec_stmt:
       eval_expr ge sp e m a v ->
       exec_stmt f sp e m (Sreturn (Some a)) E0 e m (Out_return (Some v))
   | exec_Stailcall:
-      forall f sp e m sig a bl vf vargs fd t m' m'' vres,
+      forall f sp e m sig a bl vf vargs fd t cp m' m'' vres,
       eval_expr ge (Vptr sp Ptrofs.zero) e m a vf ->
       eval_exprlist ge (Vptr sp Ptrofs.zero) e m bl vargs ->
       Genv.find_funct ge vf = Some fd ->
@@ -848,7 +858,7 @@ with exec_stmt:
       forall (COMP: comp_of fd = f.(fn_comp)),
       forall (ALLOWED: needs_calling_comp f.(fn_comp) = false),
       forall ALLOWED': Policy.allowed_call pol f.(fn_comp) fd,
-      Mem.free m sp 0 f.(fn_stackspace) = Some m' ->
+      Mem.free m sp 0 f.(fn_stackspace) cp = Some m' ->
       eval_funcall f.(fn_comp) m' fd vargs t m'' vres ->
       exec_stmt f (Vptr sp Ptrofs.zero) e m (Stailcall sig a bl) t e m'' (Out_tailcall_return vres).
 
@@ -918,7 +928,7 @@ with execinf_stmt:
       execinf_stmt f sp e m s t ->
       execinf_stmt f sp e m (Sblock s) t
   | execinf_Stailcall:
-      forall f sp e m sig a bl vf vargs fd m' t,
+      forall f sp e m sig a bl vf vargs fd cp m' t,
       eval_expr ge (Vptr sp Ptrofs.zero) e m a vf ->
       eval_exprlist ge (Vptr sp Ptrofs.zero) e m bl vargs ->
       Genv.find_funct ge vf = Some fd ->
@@ -926,7 +936,7 @@ with execinf_stmt:
       forall (COMP: comp_of fd = f.(fn_comp)),
       forall (ALLOWED: needs_calling_comp f.(fn_comp) = false),
       forall ALLOWED': Policy.allowed_call pol f.(fn_comp) fd,
-      Mem.free m sp 0 f.(fn_stackspace) = Some m' ->
+      Mem.free m sp 0 f.(fn_stackspace) cp = Some m' ->
       evalinf_funcall  m' fd vargs t ->
       execinf_stmt f (Vptr sp Ptrofs.zero) e m (Stailcall sig a bl) t.
 
@@ -1030,10 +1040,10 @@ Proof.
   eapply star_trans. eexact A.
   inversion B; clear B; subst out; simpl in H3; simpl; try contradiction.
   (* Out normal *)
-  subst vres. apply star_one. apply step_skip_call; auto.
+  subst vres. apply star_one. eapply step_skip_call; eauto.
   (* Out_return None *)
   subst vres. replace k with (call_cont k') by congruence.
-  apply star_one. apply step_return_0; auto.
+  apply star_one. eapply step_return_0; eauto.
   (* Out_return Some *)
   subst vres.
   replace k with (call_cont k') by congruence.
