backend/RTL.v
@@ -223,17 +223,17 @@ Inductive step: state -> trace -> state -> Prop :=
       step (State s f sp pc rs m)
         E0 (State s f sp pc' (rs#res <- v) m)
   | exec_Iload:
-      forall s f sp pc rs m chunk addr args dst pc' a v,
+      forall s f sp pc rs m chunk addr args dst pc' a cp v,
       (fn_code f)!pc = Some(Iload chunk addr args dst pc') ->
       eval_addressing ge sp addr rs##args = Some a ->
-      Mem.loadv chunk m a = Some v ->
+      Mem.loadv chunk m a cp = Some v ->
       step (State s f sp pc rs m)
         E0 (State s f sp pc' (rs#dst <- v) m)
   | exec_Istore:
-      forall s f sp pc rs m chunk addr args src pc' a m',
+      forall s f sp pc rs m chunk addr args src pc' a cp m',
       (fn_code f)!pc = Some(Istore chunk addr args src pc') ->
       eval_addressing ge sp addr rs##args = Some a ->
-      Mem.storev chunk m a rs#src = Some m' ->
+      Mem.storev chunk m a rs#src cp = Some m' ->
       step (State s f sp pc rs m)
         E0 (State s f sp pc' rs m')
   | exec_Icall:
@@ -245,14 +245,14 @@ Inductive step: state -> trace -> state -> Prop :=
       step (State s f sp pc rs m)
         E0 (Callstate (Stackframe res f sp pc' rs :: s) fd rs##args m)
   | exec_Itailcall:
-      forall s f stk pc rs m sig ros args fd m',
+      forall s f stk pc rs m sig ros args fd cp m',
       (fn_code f)!pc = Some(Itailcall sig ros args) ->
       find_function ros rs = Some fd ->
       funsig fd = sig ->
       forall COMP: comp_of fd = f.(fn_comp),
       forall ALLOWED: needs_calling_comp f.(fn_comp) = false,
       forall (ALLOWED': Policy.allowed_call pol f.(fn_comp) fd),
-      Mem.free m stk 0 f.(fn_stacksize) = Some m' ->
+      Mem.free m stk 0 f.(fn_stacksize) cp = Some m' ->
       step (State s f (Vptr stk Ptrofs.zero) pc rs m)
         E0 (Callstate s fd rs##args m')
   | exec_Ibuiltin:
@@ -277,9 +277,9 @@ Inductive step: state -> trace -> state -> Prop :=
       step (State s f sp pc rs m)
         E0 (State s f sp pc' rs m)
   | exec_Ireturn:
-      forall s f stk pc rs m or m',
+      forall s f stk pc rs m or cp m',
       (fn_code f)!pc = Some(Ireturn or) ->
-      Mem.free m stk 0 f.(fn_stacksize) = Some m' ->
+      Mem.free m stk 0 f.(fn_stacksize) cp = Some m' ->
       step (State s f (Vptr stk Ptrofs.zero) pc rs m)
         E0 (Returnstate s (regmap_optget or Vundef rs) m')
   | exec_function_internal:
@@ -314,10 +314,10 @@ Proof.
 Qed.
 
 Lemma exec_Iload':
-  forall s f sp pc rs m chunk addr args dst pc' rs' a v,
+  forall s f sp pc rs m chunk addr args dst pc' rs' a cp v,
   (fn_code f)!pc = Some(Iload chunk addr args dst pc') ->
   eval_addressing ge sp addr rs##args = Some a ->
-  Mem.loadv chunk m a = Some v ->
+  Mem.loadv chunk m a cp = Some v ->
   rs' = (rs#dst <- v) ->
   step (State s f sp pc rs m)
     E0 (State s f sp pc' rs' m).
